examples/knot/KnotMain0.v
@@ -47,7 +47,7 @@ Section PROOF.
 
   Definition Main: Mod.t := {|
     Mod.get_modsem := fun skenv => MainSem (Sk.load_skenv skenv);
-    Mod.sk := [("fib", Sk.Gfun)];
+    Mod.sk := [("fib", Gfun↑)];
   |}
   .
 End PROOF.
