mem/Mem1.v
@@ -9,6 +9,7 @@ Require Import PCM.
 Require Import HoareDef STB.
 Require Import ProofMode.
 
+
 Set Implicit Arguments.
 
 
@@ -85,9 +86,10 @@ Section PROOF.
     fun blk ofs =>
       match List.nth_error sk blk with
       | Some (g, gd) =>
-        match gd with
-        | Sk.Gfun => ε
-        | Sk.Gvar gv => if csl g then if (dec ofs 0%Z) then Some (Vint gv) else ε else ε
+        match gd↓ with
+        | Some Gfun => ε
+        | Some (Gvar gv) => if csl g then if (dec ofs 0%Z) then Some (Vint gv) else ε else ε
+        | _ => ε
         end
       | _ => ε
       end.
